optimistic

IMPHOL_sepref.thy
@@ -1,12 +1,79 @@
-theory IMPHOL_sepref
+theory IMPHOL_sepref                             
 imports Sepreftime "../Imperative_HOL_Time/SepLogicTime/SepAuto"
-begin      
+begin                                                       
+
+ 
 
 text \<open>Straightforward definition of refinement from
       nrest Monad to Imperative HOL (with time!).  \<close>
-definition "\<And>T. hn_refineT \<Gamma> T c \<Gamma>' R m \<equiv> nofailT m \<longrightarrow>
-  <\<Gamma> * $T> c <\<lambda>r. \<Gamma>' * (\<exists>\<^sub>Ax. R x r * \<up>(REST [x\<mapsto>T] \<le> m)) >\<^sub>t" 
+definition "\<And>T. hn_refineT \<Gamma> c \<Gamma>' R m \<equiv> nofailT m \<longrightarrow> (\<exists>T.
+  <\<Gamma> * $T> c <\<lambda>r. \<Gamma>' * (\<exists>\<^sub>Ax. R x r * \<up>(REST [x\<mapsto>T] \<le> m)) >\<^sub>t)" 
 (* maybe T should be hidden/existentially quantified *)
+
+lemma "P\<noteq>false \<Longrightarrow> \<not>(<P> c <\<lambda>_. false>)"
+  oops
+  
+
+lemma "<P> c <\<lambda>r. Q r * \<up>R> \<Longrightarrow> R"
+  apply (cases R)
+   apply auto
+  oops
+
+text \<open>example\<close>
+ 
+declare [[print_trace]]
+
+lemma ent_p: "(b \<Longrightarrow> emp \<Longrightarrow>\<^sub>A P) \<Longrightarrow> (\<up> b \<Longrightarrow>\<^sub>A P)" 
+  using entails_pure' by blast  
+
+lemma entails_ex_post': "(P \<Longrightarrow>\<^sub>A Q x) \<Longrightarrow> (P \<Longrightarrow>\<^sub>A (\<exists>\<^sub>Ax. Q x)) " 
+  using entails_ex_post by auto 
+thm entails_pure_post
+lemma entails_pure_post': "P \<Longrightarrow>\<^sub>A Q \<Longrightarrow>  b \<Longrightarrow> (P \<Longrightarrow>\<^sub>A Q * \<up> b)"
+  using entails_pure_post by blast 
+
+lemma reor: "\<up> b * true = true * \<up> b"  
+  by (simp add: assn_times_comm)
+lemma reor2: "\<up> b * \<up> q = \<up> (b \<and> q)"    
+  by (simp add: pure_conj)
+
+lemma pullin23: "\<And>P P'.  (\<exists>\<^sub>Ax. P x) * P' = (\<exists>\<^sub>Ax. P x * P') " sorry 
+
+lemma "hn_refineT emp (return 1) emp (\<lambda>x r. emp * \<up>(r=x)) (SPECT [1 \<mapsto> 1])"
+  unfolding hn_refineT_def apply auto
+  apply(rule exI[where x=1]) 
+  apply(rule post_rule)
+   apply(rule return_rule)
+  apply auto
+  apply (auto intro!: ent_p entails_ex_post'   entails_pure_post'  simp: entails_true pullin23 reor reor2 )
+  by (auto simp: one_enat_def)
+
+definition "RETURNT1 x = SPECT [x \<mapsto> 1]"
+(*
+
+lemma nres_bind_left_identity[simp]: "bindT (RETURNT1 x) f = f x"
+  unfolding bindT_def RETURNT_def 
+  by(auto split: nrest.split ) 
+
+lemma nres_bind_right_identity[simp]: "bindT M RETURNT = M" 
+  by(auto intro!: pw_eqI simp: refine_pw_simps) 
+
+lemma nres_bind_assoc[simp]: "bindT (bindT M (\<lambda>x. f x)) g = bindT M (%x. bindT (f x) g)"
+  apply(auto intro!: pw_eqI simp:  refine_pw_simps)  
+  using inresT_mono by fastforce+
+*)
+
+
+lemma "hn_refineT emp (return 1) emp (\<lambda>x r. emp * \<up>(r=x)) (SPECT [1 \<mapsto> 1])"
+  unfolding hn_refineT_def apply auto
+  apply(rule exI[where x=1]) 
+  apply(rule post_rule)
+   apply(rule return_rule)
+  apply auto
+ (* apply (auto intro!: ent_p) *)
+   by (smt One_nat_def entail_trans2 entails_ex_post entails_pure_post entails_triv entails_true one_enat_def order_mono_setup.refl)
+ 
+
 
 
 text \<open>We tag every refinement assertion with the tag @{text hn_ctxt}, to
@@ -18,12 +85,27 @@ definition hn_ctxt :: "('a\<Rightarrow>'c\<Rightarrow>assn) \<Rightarrow> 'a \<R
   "\<And>P. hn_ctxt P a c \<equiv> P a c"
 
 
+lemma entailsI: 
+  assumes "\<And>h. h\<Turnstile>P \<Longrightarrow> h\<Turnstile>Q"
+  shows "P \<Longrightarrow>\<^sub>A Q"            
+  using assms unfolding entails_def by auto
+
+
+lemma mod_star_trueI: "h\<Turnstile>P \<Longrightarrow> h\<Turnstile>P*true"   
+  by (metis assn_times_comm entailsD' entails_true mult.left_neutral)
+
 subsubsection \<open>Weak Entails\<close>    
 text \<open>Weakening of entails to allow arbitrary unspecified memory in conclusion\<close>
 definition entailst :: "assn \<Rightarrow> assn \<Rightarrow> bool" (infix "\<Longrightarrow>\<^sub>t" 10)
   where "entailst A B \<equiv> A \<Longrightarrow>\<^sub>A B * true"
 
+lemma enttI: "A\<Longrightarrow>\<^sub>AB*true \<Longrightarrow> A\<Longrightarrow>\<^sub>tB" unfolding entailst_def .
 lemma enttD: "A\<Longrightarrow>\<^sub>tB \<Longrightarrow> A\<Longrightarrow>\<^sub>AB*true" unfolding entailst_def .
+
+lemma entt_refl[simp, intro!]: "entailst A A"
+  unfolding entailst_def
+  by (simp add: entailsI mod_star_trueI)
+ 
 
 
 lemma ent_frame_fwd: fixes P
@@ -41,7 +123,6 @@ lemma normalize_rules: "\<And>P. (\<And>x. <P x> f <Q>) \<Longrightarrow> <\<exi
 
 lemma pullin: "\<And>P. <\<exists>\<^sub>Ax. P' * P x> f <Q> \<Longrightarrow> <P' * (\<exists>\<^sub>Ax. P x)> f <Q>" sorry 
 lemma pullin2: "\<And>P P'. P' * (\<exists>\<^sub>Ax. P x) = (\<exists>\<^sub>Ax. P' * P x) " sorry 
-lemma pullin23: "\<And>P P'.  (\<exists>\<^sub>Ax. P x) * P' = (\<exists>\<^sub>Ax. P x * P') " sorry 
 lemma pullia: "\<And>P. Q * ((\<exists>\<^sub>Ax. P x) * (R::assn)) = (\<exists>\<^sub>Ax. P x) * (Q * (R::assn))" sorry
 lemma pullia2: "\<And>P. (Q * (\<exists>\<^sub>Ax. P x)) * (R::assn) = (\<exists>\<^sub>Ax. P x) * (Q * (R::assn))" sorry
 lemma pullia3: "\<And>P. (Q * (\<exists>\<^sub>Ax. P x)) * (R::assn) = (Q * (R::assn)) * (\<exists>\<^sub>Ax. P x)" sorry
@@ -81,7 +162,7 @@ lemma ent_ex_postI: "\<And>P. (P \<Longrightarrow>\<^sub>A Q x) \<Longrightarrow
 
 declare [[print_trace]]
 
-lemma hnr_bind:
+(*lemma hnr_bind:
   assumes D1: "hn_refineT \<Gamma> T1 m' \<Gamma>1 Rh m"
   assumes D2: 
     "\<And>x x'. SPECT [x \<mapsto> enat T1] \<le> m \<Longrightarrow> hn_refineT (\<Gamma>1 * hn_ctxt Rh x x') T2 (f' x') (\<Gamma>2 x x') R (f x)"
@@ -150,14 +231,93 @@ proof -
       by (smt assn_times_comm entails_def mod_pure_star_dist mult.left_commute top_assn_reduce)
     done
 qed
+*)
+
+lemma hnr_bind:
+  assumes D1: "hn_refineT \<Gamma>  m' \<Gamma>1 Rh m"
+  assumes D2: 
+    "\<And>x x'. RETURNT  x \<le> m \<Longrightarrow> hn_refineT (\<Gamma>1 * hn_ctxt Rh x x')  (f' x') (\<Gamma>2 x x') R (f x)"
+  assumes IMP: "\<And>x x'. \<Gamma>2 x x' \<Longrightarrow>\<^sub>t \<Gamma>' * hn_ctxt Rx x x'" 
+  shows "hn_refineT \<Gamma> (m'\<bind>f') \<Gamma>' R (m\<bind>f)"  
+  using assms
+  unfolding hn_refineT_def
+  apply (clarsimp simp add: pw_bindT_nofailT)
+  subgoal for T1 
+    apply rule 
+  apply(rule SepAuto.bind_rule)
+  apply(subst time_credit_add)
+  apply(subst assn_times_assoc[symmetric])
+  apply(rule frame_rule)
+  apply assumption
+  apply (clarsimp    simp: hn_ctxt_def)
+  apply(clarsimp simp: pullia3 ) apply(clarsimp simp: pullin2) 
+  apply(clarsimp intro!: normalize_rules)
+  apply(clarsimp simp: assn_times_assoc[symmetric])
+  apply(clarsimp intro!: normalize_rules)
+proof -
+  fix x' x
+    
+
+  assume 1: "SPECT [x \<mapsto> enat T1] \<le> m" 
+    and "nofailT m" "\<forall>x. (\<exists>t. inresT m x t)  \<longrightarrow> nofailT (f x)"
+  hence "nofailT (f x)" "RETURNT x \<le> m"   by (auto simp: pw_le_iff split: if_splits)
+  moreover assume "\<And>x x'. RETURNT x \<le> m \<Longrightarrow>
+           nofailT (f x) \<longrightarrow> (\<exists>T2.  <\<Gamma>1 * Rh x x' * $ T2> f' x'
+           <\<lambda>r'. \<exists>\<^sub>Ar. \<Gamma>2 x x' * true * R r r' * \<up> (SPECT [r \<mapsto> enat T2] \<le> f x)>)"
+  ultimately have "\<And>x'. \<exists>T2. <\<Gamma>1 * Rh x x'* $ T2> f' x'
+           <\<lambda>r'. \<exists>\<^sub>Ar. \<Gamma>2 x x' * true * R r r' * \<up> (SPECT [r \<mapsto> enat T2] \<le> f x)>"
+    by simp
+  then obtain T2 where "<\<Gamma>1 * Rh x x'* $ T2> f' x'
+           <\<lambda>r'. \<exists>\<^sub>Ar. \<Gamma>2 x x' * true * R r r' * \<up> (SPECT [r \<mapsto> enat T2] \<le> f x)>" by auto
+  also
 
 
+  have  f: "\<And>r r'. \<Gamma>2 x x' * true * R r' r * \<up> (SPECT [r' \<mapsto> enat T2] \<le> f x)
+      = \<Gamma>2 x x' * (true * R r' r * \<up> (SPECT [r' \<mapsto> enat T2] \<le> f x))"
+     by (simp add: assn_times_assoc) 
 
+   have k: "RETURNT x \<le> SPECT [x \<mapsto> enat T1]" unfolding RETURNT_def apply auto   
+     by (simp add:  le_fun_def)
+
+  have "\<And>r'. \<exists>\<^sub>Ar. \<Gamma>2 x x' * true * R r r' * \<up> (SPECT [r \<mapsto> enat T2] \<le> f x) \<Longrightarrow>\<^sub>A
+    \<exists>\<^sub>Ar. \<Gamma>' * R r r' * true * \<up> (SPECT [r \<mapsto> enat T2] \<le> f x)" 
+    apply(intro ent_ex_preI )
+    subgoal for r r'
+    apply(intro ent_ex_postI[where x=r'])   
+      apply(rule ent_frame_fwd[OF IMP[THEN enttD]]) 
+      unfolding f
+       apply(rule entails_frame[where R="true * R r' r * \<up> (SPECT [r' \<mapsto> enat T2] \<le> f x)"])
+       apply(rule entails_triv)
+      by auto2
+    done
+  finally (cons_post_rule) have 
+    R: "<\<Gamma>1 * Rh x x' * $T2> f' x' 
+        <\<lambda>r'. \<exists>\<^sub>Ar. \<Gamma>' * R r r' * true * \<up>(SPECT [r \<mapsto> enat T2] \<le> f x)>"
+    .
+  have g: "\<Gamma>1 * true * $ T2 * Rh x x' = (\<Gamma>1   * Rh x x' * $ T2) * true"  
+    using assn_times_assoc assn_times_comm by auto 
+
+  have "<\<Gamma>1 * true * $ T2 * Rh x x'> f' x'
+          <\<lambda>r. \<exists>\<^sub>Ax. \<Gamma>' * true * R x r * \<up> (SPECT [x \<mapsto> enat (T1 + T2)] \<le> m \<bind> f)>"
+    unfolding g
+    apply(rule post_rule) 
+     apply(rule frame_rule) 
+     apply(rule R) 
+    apply(simp add: pullin23)
+    apply safe 
+    apply(intro ent_ex_preI )
+    subgoal for r r'
+    apply(intro ent_ex_postI[where x=r']) 
+      using bind_det_aux[OF 1]  
+      by (smt assn_times_comm entails_def mod_pure_star_dist mult.left_commute top_assn_reduce)
+    done 
+       show "<\<Gamma>1 * true * $ T2 * Rh x x'> f' x' <\<lambda>r. \<exists>\<^sub>Ax. \<Gamma>' * true * R x r * \<up> (SPECT [x \<mapsto> enat (T1 + T2)] \<le> m \<bind> f)>"
+  qed 
 
 lemma hnr_frame: fixes P T
-  assumes "hn_refineT P' T1 c Q' R m"
+  assumes "hn_refineT P'  c Q' R m"
   assumes "P \<Longrightarrow>\<^sub>t F * P'"
-  shows "hn_refineT P T1 c (F * Q') R m"
+  shows "hn_refineT P  c (F * Q') R m"
   using assms
   unfolding hn_refineT_def entailst_def
   apply clarsimp  (*
@@ -169,46 +329,46 @@ lemma hnr_frame: fixes P T
   done *)
 sorry
 
-lemma hnr_cons: fixes P T
+lemma hnr_cons: 
   assumes I: "P\<Longrightarrow>\<^sub>tP'"
-  assumes R: "hn_refineT P' T c Q R m"
+  assumes R: "hn_refineT P'  c Q R m"
   assumes I': "Q\<Longrightarrow>\<^sub>tQ'"
   assumes R': "\<And>x y. R x y \<Longrightarrow>\<^sub>t R' x y"
-  shows "hn_refineT P T c Q' R' m"
+  shows "hn_refineT P  c Q' R' m"
   sorry
 
 
 lemma hn_refineI[intro?]: fixes T
   assumes "nofailT m 
-    \<Longrightarrow> <\<Gamma> * $ T> c <\<lambda>r. \<Gamma>' * (\<exists>\<^sub>Ax. R x r * \<up> (SPECT [x \<mapsto> enat T] \<le> m))>\<^sub>t"
-  shows "hn_refineT \<Gamma> T  c \<Gamma>' R m"
+    \<Longrightarrow> (\<exists>T. <\<Gamma> * $ T> c <\<lambda>r. \<Gamma>' * (\<exists>\<^sub>Ax. R x r * \<up> (SPECT [x \<mapsto> enat T] \<le> m))>\<^sub>t)"
+  shows "hn_refineT \<Gamma>   c \<Gamma>' R m"
   using assms unfolding hn_refineT_def by blast
 
 lemma hn_refineD: fixes T
-  assumes "hn_refineT \<Gamma> T c \<Gamma>' R m"
+  assumes "hn_refineT \<Gamma> c \<Gamma>' R m"
   assumes "nofailT  m"
-  shows " <\<Gamma> * $ T> c <\<lambda>r. \<Gamma>' * (\<exists>\<^sub>Ax. R x r * \<up> (SPECT [x \<mapsto> enat T] \<le> m))>\<^sub>t"
+  shows "(\<exists>T. <\<Gamma> * $ T> c <\<lambda>r. \<Gamma>' * (\<exists>\<^sub>Ax. R x r * \<up> (SPECT [x \<mapsto> enat T] \<le> m))>\<^sub>t)"
   using assms unfolding hn_refineT_def by blast
 
 lemma hnr_ref: fixes P T
   assumes LE: "m\<le>m'"
-  assumes R: "hn_refineT P T c Q R m"
-  shows "hn_refineT P T c Q R m'"
-  apply rule
+  assumes R: "hn_refineT P  c Q R m"
+  shows "hn_refineT P  c Q R m'"
+  apply rule  (*
   apply (rule cons_post_rule)
   apply (rule hn_refineD[OF R])
   using LE apply (simp add: pw_le_iff)
   using LE apply auto2 
-  done
+  done *) sorry
 
 
 lemma hn_refineT_cons_complete: fixes P T
   assumes I: "P\<Longrightarrow>\<^sub>tP'"
-  assumes R: "hn_refineT P' T c Q R m"
+  assumes R: "hn_refineT P' c Q R m"
   assumes I': "Q\<Longrightarrow>\<^sub>tQ'"
   assumes R': "\<And>x y. R x y \<Longrightarrow>\<^sub>t R' x y"
   assumes LE: "m\<le>m'"
-  shows "hn_refineT P T c Q' R' m'"
+  shows "hn_refineT P  c Q' R' m'"
   apply (rule hnr_ref[OF LE])
   apply (rule hnr_cons[OF I R I' R'])
   done
